AwsCryptographicMaterialProviders/runtimes/java/src/main/smithy-generated/software/amazon/cryptography/keystore/model/QueryForVersionsInput.java
@@ -1,0 +1,176 @@
+// Copyright Amazon.com Inc. or its affiliates. All Rights Reserved.
+// SPDX-License-Identifier: Apache-2.0
+// Do not modify this file. This file is machine generated, and any changes to it will be overwritten.
+package software.amazon.cryptography.keystore.model;
+
+import java.nio.ByteBuffer;
+import java.util.Objects;
+
+public class QueryForVersionsInput {
+
+  /**
+   * Optional.
+   *   If set, Query will start at this index and read forward.
+   *   Otherwise, Query will start at the indexes begining.
+   *   The Default Storage is DDB;
+   *   see Amazon DynamoDB's defination of exclusiveStartKey for details.
+   *   Note: While the Default Storage is DDB,
+   *   the Key Store transforms the exclusiveStartKey into an opaque representation.
+   */
+  private final ByteBuffer exclusiveStartKey;
+
+  /**
+   * The Identifier of the Branch Key.
+   */
+  private final String Identifier;
+
+  /**
+   * The maximum read items.
+   */
+  private final Integer pageSize;
+
+  protected QueryForVersionsInput(BuilderImpl builder) {
+    this.exclusiveStartKey = builder.exclusiveStartKey();
+    this.Identifier = builder.Identifier();
+    this.pageSize = builder.pageSize();
+  }
+
+  /**
+   * @return Optional.
+   *   If set, Query will start at this index and read forward.
+   *   Otherwise, Query will start at the indexes begining.
+   *   The Default Storage is DDB;
+   *   see Amazon DynamoDB's defination of exclusiveStartKey for details.
+   *   Note: While the Default Storage is DDB,
+   *   the Key Store transforms the exclusiveStartKey into an opaque representation.
+   */
+  public ByteBuffer exclusiveStartKey() {
+    return this.exclusiveStartKey;
+  }
+
+  /**
+   * @return The Identifier of the Branch Key.
+   */
+  public String Identifier() {
+    return this.Identifier;
+  }
+
+  /**
+   * @return The maximum read items.
+   */
+  public Integer pageSize() {
+    return this.pageSize;
+  }
+
+  public Builder toBuilder() {
+    return new BuilderImpl(this);
+  }
+
+  public static Builder builder() {
+    return new BuilderImpl();
+  }
+
+  public interface Builder {
+    /**
+     * @param exclusiveStartKey Optional.
+     *   If set, Query will start at this index and read forward.
+     *   Otherwise, Query will start at the indexes begining.
+     *   The Default Storage is DDB;
+     *   see Amazon DynamoDB's defination of exclusiveStartKey for details.
+     *   Note: While the Default Storage is DDB,
+     *   the Key Store transforms the exclusiveStartKey into an opaque representation.
+     */
+    Builder exclusiveStartKey(ByteBuffer exclusiveStartKey);
+
+    /**
+     * @return Optional.
+     *   If set, Query will start at this index and read forward.
+     *   Otherwise, Query will start at the indexes begining.
+     *   The Default Storage is DDB;
+     *   see Amazon DynamoDB's defination of exclusiveStartKey for details.
+     *   Note: While the Default Storage is DDB,
+     *   the Key Store transforms the exclusiveStartKey into an opaque representation.
+     */
+    ByteBuffer exclusiveStartKey();
+
+    /**
+     * @param Identifier The Identifier of the Branch Key.
+     */
+    Builder Identifier(String Identifier);
+
+    /**
+     * @return The Identifier of the Branch Key.
+     */
+    String Identifier();
+
+    /**
+     * @param pageSize The maximum read items.
+     */
+    Builder pageSize(Integer pageSize);
+
+    /**
+     * @return The maximum read items.
+     */
+    Integer pageSize();
+
+    QueryForVersionsInput build();
+  }
+
+  static class BuilderImpl implements Builder {
+
+    protected ByteBuffer exclusiveStartKey;
+
+    protected String Identifier;
+
+    protected Integer pageSize;
+
+    protected BuilderImpl() {}
+
+    protected BuilderImpl(QueryForVersionsInput model) {
+      this.exclusiveStartKey = model.exclusiveStartKey();
+      this.Identifier = model.Identifier();
+      this.pageSize = model.pageSize();
+    }
+
+    public Builder exclusiveStartKey(ByteBuffer exclusiveStartKey) {
+      this.exclusiveStartKey = exclusiveStartKey;
+      return this;
+    }
+
+    public ByteBuffer exclusiveStartKey() {
+      return this.exclusiveStartKey;
+    }
+
+    public Builder Identifier(String Identifier) {
+      this.Identifier = Identifier;
+      return this;
+    }
+
+    public String Identifier() {
+      return this.Identifier;
+    }
+
+    public Builder pageSize(Integer pageSize) {
+      this.pageSize = pageSize;
+      return this;
+    }
+
+    public Integer pageSize() {
+      return this.pageSize;
+    }
+
+    public QueryForVersionsInput build() {
+      if (Objects.isNull(this.Identifier())) {
+        throw new IllegalArgumentException(
+          "Missing value for required field `Identifier`"
+        );
+      }
+      if (Objects.isNull(this.pageSize())) {
+        throw new IllegalArgumentException(
+          "Missing value for required field `pageSize`"
+        );
+      }
+      return new QueryForVersionsInput(this);
+    }
+  }
+}
