AwsCryptographicMaterialProviders/runtimes/java/src/main/smithy-generated/software/amazon/cryptography/keystore/model/QueryForVersionsOutput.java
@@ -1,0 +1,138 @@
+// Copyright Amazon.com Inc. or its affiliates. All Rights Reserved.
+// SPDX-License-Identifier: Apache-2.0
+// Do not modify this file. This file is machine generated, and any changes to it will be overwritten.
+package software.amazon.cryptography.keystore.model;
+
+import java.nio.ByteBuffer;
+import java.util.List;
+import java.util.Objects;
+
+public class QueryForVersionsOutput {
+
+  /**
+   * If none-empty, Query did not finish searching storage.
+   *   Next Query should resume from here.
+   *   The Default Storage is DDB;
+   *   see Amazon DynamoDB's defination of exclusiveStartKey for details.
+   *   Note: While the Default Storage is DDB,
+   *   the Key Store transforms the exclusiveStartKey into an opaque representation.
+   */
+  private final ByteBuffer exclusiveStartKey;
+
+  /**
+   * Up to pageSize list of version (decrypt only) items of a Branch Key.
+   */
+  private final List<EncryptedHierarchicalKey> items;
+
+  protected QueryForVersionsOutput(BuilderImpl builder) {
+    this.exclusiveStartKey = builder.exclusiveStartKey();
+    this.items = builder.items();
+  }
+
+  /**
+   * @return If none-empty, Query did not finish searching storage.
+   *   Next Query should resume from here.
+   *   The Default Storage is DDB;
+   *   see Amazon DynamoDB's defination of exclusiveStartKey for details.
+   *   Note: While the Default Storage is DDB,
+   *   the Key Store transforms the exclusiveStartKey into an opaque representation.
+   */
+  public ByteBuffer exclusiveStartKey() {
+    return this.exclusiveStartKey;
+  }
+
+  /**
+   * @return Up to pageSize list of version (decrypt only) items of a Branch Key.
+   */
+  public List<EncryptedHierarchicalKey> items() {
+    return this.items;
+  }
+
+  public Builder toBuilder() {
+    return new BuilderImpl(this);
+  }
+
+  public static Builder builder() {
+    return new BuilderImpl();
+  }
+
+  public interface Builder {
+    /**
+     * @param exclusiveStartKey If none-empty, Query did not finish searching storage.
+     *   Next Query should resume from here.
+     *   The Default Storage is DDB;
+     *   see Amazon DynamoDB's defination of exclusiveStartKey for details.
+     *   Note: While the Default Storage is DDB,
+     *   the Key Store transforms the exclusiveStartKey into an opaque representation.
+     */
+    Builder exclusiveStartKey(ByteBuffer exclusiveStartKey);
+
+    /**
+     * @return If none-empty, Query did not finish searching storage.
+     *   Next Query should resume from here.
+     *   The Default Storage is DDB;
+     *   see Amazon DynamoDB's defination of exclusiveStartKey for details.
+     *   Note: While the Default Storage is DDB,
+     *   the Key Store transforms the exclusiveStartKey into an opaque representation.
+     */
+    ByteBuffer exclusiveStartKey();
+
+    /**
+     * @param items Up to pageSize list of version (decrypt only) items of a Branch Key.
+     */
+    Builder items(List<EncryptedHierarchicalKey> items);
+
+    /**
+     * @return Up to pageSize list of version (decrypt only) items of a Branch Key.
+     */
+    List<EncryptedHierarchicalKey> items();
+
+    QueryForVersionsOutput build();
+  }
+
+  static class BuilderImpl implements Builder {
+
+    protected ByteBuffer exclusiveStartKey;
+
+    protected List<EncryptedHierarchicalKey> items;
+
+    protected BuilderImpl() {}
+
+    protected BuilderImpl(QueryForVersionsOutput model) {
+      this.exclusiveStartKey = model.exclusiveStartKey();
+      this.items = model.items();
+    }
+
+    public Builder exclusiveStartKey(ByteBuffer exclusiveStartKey) {
+      this.exclusiveStartKey = exclusiveStartKey;
+      return this;
+    }
+
+    public ByteBuffer exclusiveStartKey() {
+      return this.exclusiveStartKey;
+    }
+
+    public Builder items(List<EncryptedHierarchicalKey> items) {
+      this.items = items;
+      return this;
+    }
+
+    public List<EncryptedHierarchicalKey> items() {
+      return this.items;
+    }
+
+    public QueryForVersionsOutput build() {
+      if (Objects.isNull(this.exclusiveStartKey())) {
+        throw new IllegalArgumentException(
+          "Missing value for required field `exclusiveStartKey`"
+        );
+      }
+      if (Objects.isNull(this.items())) {
+        throw new IllegalArgumentException(
+          "Missing value for required field `items`"
+        );
+      }
+      return new QueryForVersionsOutput(this);
+    }
+  }
+}
