AwsCryptographicMaterialProviders/runtimes/java/src/main/smithy-generated/software/amazon/cryptography/keystore/model/WriteInitializeMutationInput.java
@@ -1,0 +1,300 @@
+// Copyright Amazon.com Inc. or its affiliates. All Rights Reserved.
+// SPDX-License-Identifier: Apache-2.0
+// Do not modify this file. This file is machine generated, and any changes to it will be overwritten.
+package software.amazon.cryptography.keystore.model;
+
+import java.util.Objects;
+
+public class WriteInitializeMutationInput {
+
+  /**
+   *
+   *   The active representation of this branch key,
+   *   generated with the Mutation's terminal properities.
+   *   The plain-text cryptographic material of the Active must be the same as the Version.
+   */
+  private final EncryptedHierarchicalKey active;
+
+  /**
+   *
+   *   The previous active version.
+   *   This key should be used as an optimistic lock on the new version.
+   *   This means that when updating the current active record
+   *   the existing active record should be equal to this value.
+   */
+  private final EncryptedHierarchicalKey oldActive;
+
+  /**
+   *
+   *   The decrypt representation of this branch key version,
+   *   generated with the Mutation's terminal properities.
+   *   The plain-text cryptographic material of the `Version` must be the same as the `Active`.
+   */
+  private final EncryptedHierarchicalKey version;
+
+  /**
+   *
+   *   The mutated HMAC key used to support searchable encryption.
+   *   The cryptographic material is identical to the existing beacon,
+   *   but is now authorized with the Mutation's terminal properities.
+   */
+  private final EncryptedHierarchicalKey beacon;
+
+  /**
+   * Information an in-flight Mutation of a Branch Key.
+   * This ensures:
+   * - only one Mutation affects a Branch Key at a time
+   * - all items of a Branch Key are mutated consistently
+   */
+  private final MutationLock mutationLock;
+
+  protected WriteInitializeMutationInput(BuilderImpl builder) {
+    this.active = builder.active();
+    this.oldActive = builder.oldActive();
+    this.version = builder.version();
+    this.beacon = builder.beacon();
+    this.mutationLock = builder.mutationLock();
+  }
+
+  /**
+   * @return
+   *   The active representation of this branch key,
+   *   generated with the Mutation's terminal properities.
+   *   The plain-text cryptographic material of the Active must be the same as the Version.
+   */
+  public EncryptedHierarchicalKey active() {
+    return this.active;
+  }
+
+  /**
+   * @return
+   *   The previous active version.
+   *   This key should be used as an optimistic lock on the new version.
+   *   This means that when updating the current active record
+   *   the existing active record should be equal to this value.
+   */
+  public EncryptedHierarchicalKey oldActive() {
+    return this.oldActive;
+  }
+
+  /**
+   * @return
+   *   The decrypt representation of this branch key version,
+   *   generated with the Mutation's terminal properities.
+   *   The plain-text cryptographic material of the `Version` must be the same as the `Active`.
+   */
+  public EncryptedHierarchicalKey version() {
+    return this.version;
+  }
+
+  /**
+   * @return
+   *   The mutated HMAC key used to support searchable encryption.
+   *   The cryptographic material is identical to the existing beacon,
+   *   but is now authorized with the Mutation's terminal properities.
+   */
+  public EncryptedHierarchicalKey beacon() {
+    return this.beacon;
+  }
+
+  /**
+   * @return Information an in-flight Mutation of a Branch Key.
+   * This ensures:
+   * - only one Mutation affects a Branch Key at a time
+   * - all items of a Branch Key are mutated consistently
+   */
+  public MutationLock mutationLock() {
+    return this.mutationLock;
+  }
+
+  public Builder toBuilder() {
+    return new BuilderImpl(this);
+  }
+
+  public static Builder builder() {
+    return new BuilderImpl();
+  }
+
+  public interface Builder {
+    /**
+     * @param active
+     *   The active representation of this branch key,
+     *   generated with the Mutation's terminal properities.
+     *   The plain-text cryptographic material of the Active must be the same as the Version.
+     */
+    Builder active(EncryptedHierarchicalKey active);
+
+    /**
+     * @return
+     *   The active representation of this branch key,
+     *   generated with the Mutation's terminal properities.
+     *   The plain-text cryptographic material of the Active must be the same as the Version.
+     */
+    EncryptedHierarchicalKey active();
+
+    /**
+     * @param oldActive
+     *   The previous active version.
+     *   This key should be used as an optimistic lock on the new version.
+     *   This means that when updating the current active record
+     *   the existing active record should be equal to this value.
+     */
+    Builder oldActive(EncryptedHierarchicalKey oldActive);
+
+    /**
+     * @return
+     *   The previous active version.
+     *   This key should be used as an optimistic lock on the new version.
+     *   This means that when updating the current active record
+     *   the existing active record should be equal to this value.
+     */
+    EncryptedHierarchicalKey oldActive();
+
+    /**
+     * @param version
+     *   The decrypt representation of this branch key version,
+     *   generated with the Mutation's terminal properities.
+     *   The plain-text cryptographic material of the `Version` must be the same as the `Active`.
+     */
+    Builder version(EncryptedHierarchicalKey version);
+
+    /**
+     * @return
+     *   The decrypt representation of this branch key version,
+     *   generated with the Mutation's terminal properities.
+     *   The plain-text cryptographic material of the `Version` must be the same as the `Active`.
+     */
+    EncryptedHierarchicalKey version();
+
+    /**
+     * @param beacon
+     *   The mutated HMAC key used to support searchable encryption.
+     *   The cryptographic material is identical to the existing beacon,
+     *   but is now authorized with the Mutation's terminal properities.
+     */
+    Builder beacon(EncryptedHierarchicalKey beacon);
+
+    /**
+     * @return
+     *   The mutated HMAC key used to support searchable encryption.
+     *   The cryptographic material is identical to the existing beacon,
+     *   but is now authorized with the Mutation's terminal properities.
+     */
+    EncryptedHierarchicalKey beacon();
+
+    /**
+     * @param mutationLock Information an in-flight Mutation of a Branch Key.
+     * This ensures:
+     * - only one Mutation affects a Branch Key at a time
+     * - all items of a Branch Key are mutated consistently
+     */
+    Builder mutationLock(MutationLock mutationLock);
+
+    /**
+     * @return Information an in-flight Mutation of a Branch Key.
+     * This ensures:
+     * - only one Mutation affects a Branch Key at a time
+     * - all items of a Branch Key are mutated consistently
+     */
+    MutationLock mutationLock();
+
+    WriteInitializeMutationInput build();
+  }
+
+  static class BuilderImpl implements Builder {
+
+    protected EncryptedHierarchicalKey active;
+
+    protected EncryptedHierarchicalKey oldActive;
+
+    protected EncryptedHierarchicalKey version;
+
+    protected EncryptedHierarchicalKey beacon;
+
+    protected MutationLock mutationLock;
+
+    protected BuilderImpl() {}
+
+    protected BuilderImpl(WriteInitializeMutationInput model) {
+      this.active = model.active();
+      this.oldActive = model.oldActive();
+      this.version = model.version();
+      this.beacon = model.beacon();
+      this.mutationLock = model.mutationLock();
+    }
+
+    public Builder active(EncryptedHierarchicalKey active) {
+      this.active = active;
+      return this;
+    }
+
+    public EncryptedHierarchicalKey active() {
+      return this.active;
+    }
+
+    public Builder oldActive(EncryptedHierarchicalKey oldActive) {
+      this.oldActive = oldActive;
+      return this;
+    }
+
+    public EncryptedHierarchicalKey oldActive() {
+      return this.oldActive;
+    }
+
+    public Builder version(EncryptedHierarchicalKey version) {
+      this.version = version;
+      return this;
+    }
+
+    public EncryptedHierarchicalKey version() {
+      return this.version;
+    }
+
+    public Builder beacon(EncryptedHierarchicalKey beacon) {
+      this.beacon = beacon;
+      return this;
+    }
+
+    public EncryptedHierarchicalKey beacon() {
+      return this.beacon;
+    }
+
+    public Builder mutationLock(MutationLock mutationLock) {
+      this.mutationLock = mutationLock;
+      return this;
+    }
+
+    public MutationLock mutationLock() {
+      return this.mutationLock;
+    }
+
+    public WriteInitializeMutationInput build() {
+      if (Objects.isNull(this.active())) {
+        throw new IllegalArgumentException(
+          "Missing value for required field `active`"
+        );
+      }
+      if (Objects.isNull(this.oldActive())) {
+        throw new IllegalArgumentException(
+          "Missing value for required field `oldActive`"
+        );
+      }
+      if (Objects.isNull(this.version())) {
+        throw new IllegalArgumentException(
+          "Missing value for required field `version`"
+        );
+      }
+      if (Objects.isNull(this.beacon())) {
+        throw new IllegalArgumentException(
+          "Missing value for required field `beacon`"
+        );
+      }
+      if (Objects.isNull(this.mutationLock())) {
+        throw new IllegalArgumentException(
+          "Missing value for required field `mutationLock`"
+        );
+      }
+      return new WriteInitializeMutationInput(this);
+    }
+  }
+}
