AwsCryptographicMaterialProviders/runtimes/net/Generated/AwsCryptographyKeyStore/NativeWrapper_KeyStorageInterface.cs
@@ -45,6 +45,34 @@ namespace AWS.Cryptography.KeyStore
     {
       throw new KeyStoreException("Not supported at this time.");
     }
+    public Wrappers_Compile._IResult<software.amazon.cryptography.keystore.internaldafny.types._IWriteMutatedVersionsOutput, software.amazon.cryptography.keystore.internaldafny.types._IError> WriteMutatedVersions(software.amazon.cryptography.keystore.internaldafny.types._IWriteMutatedVersionsInput input)
+    {
+      void validateOutput(AWS.Cryptography.KeyStore.WriteMutatedVersionsOutput nativeOutput)
+      {
+        try { nativeOutput.Validate(); }
+        catch (ArgumentException e)
+        {
+          var message = $"Output of {_impl}._WriteMutatedVersions is invalid. {e.Message}";
+          throw new KeyStoreException(message);
+        }
+      }
+      AWS.Cryptography.KeyStore.WriteMutatedVersionsInput nativeInput = TypeConversion.FromDafny_N3_aws__N12_cryptography__N8_keyStore__S25_WriteMutatedVersionsInput(input);
+      try
+      {
+        AWS.Cryptography.KeyStore.WriteMutatedVersionsOutput nativeOutput = _impl.WriteMutatedVersions(nativeInput);
+        _ = nativeOutput ?? throw new KeyStoreException($"{_impl}._WriteMutatedVersions returned null, should be {typeof(AWS.Cryptography.KeyStore.WriteMutatedVersionsOutput)}");
+        validateOutput(nativeOutput);
+        return Wrappers_Compile.Result<software.amazon.cryptography.keystore.internaldafny.types._IWriteMutatedVersionsOutput, software.amazon.cryptography.keystore.internaldafny.types._IError>.create_Success(TypeConversion.ToDafny_N3_aws__N12_cryptography__N8_keyStore__S26_WriteMutatedVersionsOutput(nativeOutput));
+      }
+      catch (Exception e)
+      {
+        return Wrappers_Compile.Result<software.amazon.cryptography.keystore.internaldafny.types._IWriteMutatedVersionsOutput, software.amazon.cryptography.keystore.internaldafny.types._IError>.create_Failure(TypeConversion.ToDafny_CommonError(e));
+      }
+    }
+    public Wrappers_Compile._IResult<software.amazon.cryptography.keystore.internaldafny.types._IWriteMutatedVersionsOutput, software.amazon.cryptography.keystore.internaldafny.types._IError> WriteMutatedVersions_k(software.amazon.cryptography.keystore.internaldafny.types._IWriteMutatedVersionsInput input)
+    {
+      throw new KeyStoreException("Not supported at this time.");
+    }
     public Wrappers_Compile._IResult<software.amazon.cryptography.keystore.internaldafny.types._IWriteNewEncryptedBranchKeyOutput, software.amazon.cryptography.keystore.internaldafny.types._IError> WriteNewEncryptedBranchKey(software.amazon.cryptography.keystore.internaldafny.types._IWriteNewEncryptedBranchKeyInput input)
     {
       void validateOutput(AWS.Cryptography.KeyStore.WriteNewEncryptedBranchKeyOutput nativeOutput)
@@ -73,6 +101,62 @@ namespace AWS.Cryptography.KeyStore
     {
       throw new KeyStoreException("Not supported at this time.");
     }
+    public Wrappers_Compile._IResult<software.amazon.cryptography.keystore.internaldafny.types._IWriteInitializeMutationOutput, software.amazon.cryptography.keystore.internaldafny.types._IError> WriteInitializeMutation(software.amazon.cryptography.keystore.internaldafny.types._IWriteInitializeMutationInput input)
+    {
+      void validateOutput(AWS.Cryptography.KeyStore.WriteInitializeMutationOutput nativeOutput)
+      {
+        try { nativeOutput.Validate(); }
+        catch (ArgumentException e)
+        {
+          var message = $"Output of {_impl}._WriteInitializeMutation is invalid. {e.Message}";
+          throw new KeyStoreException(message);
+        }
+      }
+      AWS.Cryptography.KeyStore.WriteInitializeMutationInput nativeInput = TypeConversion.FromDafny_N3_aws__N12_cryptography__N8_keyStore__S28_WriteInitializeMutationInput(input);
+      try
+      {
+        AWS.Cryptography.KeyStore.WriteInitializeMutationOutput nativeOutput = _impl.WriteInitializeMutation(nativeInput);
+        _ = nativeOutput ?? throw new KeyStoreException($"{_impl}._WriteInitializeMutation returned null, should be {typeof(AWS.Cryptography.KeyStore.WriteInitializeMutationOutput)}");
+        validateOutput(nativeOutput);
+        return Wrappers_Compile.Result<software.amazon.cryptography.keystore.internaldafny.types._IWriteInitializeMutationOutput, software.amazon.cryptography.keystore.internaldafny.types._IError>.create_Success(TypeConversion.ToDafny_N3_aws__N12_cryptography__N8_keyStore__S29_WriteInitializeMutationOutput(nativeOutput));
+      }
+      catch (Exception e)
+      {
+        return Wrappers_Compile.Result<software.amazon.cryptography.keystore.internaldafny.types._IWriteInitializeMutationOutput, software.amazon.cryptography.keystore.internaldafny.types._IError>.create_Failure(TypeConversion.ToDafny_CommonError(e));
+      }
+    }
+    public Wrappers_Compile._IResult<software.amazon.cryptography.keystore.internaldafny.types._IWriteInitializeMutationOutput, software.amazon.cryptography.keystore.internaldafny.types._IError> WriteInitializeMutation_k(software.amazon.cryptography.keystore.internaldafny.types._IWriteInitializeMutationInput input)
+    {
+      throw new KeyStoreException("Not supported at this time.");
+    }
+    public Wrappers_Compile._IResult<software.amazon.cryptography.keystore.internaldafny.types._IGetItemsForInitializeMutationOutput, software.amazon.cryptography.keystore.internaldafny.types._IError> GetItemsForInitializeMutation(software.amazon.cryptography.keystore.internaldafny.types._IGetItemsForInitializeMutationInput input)
+    {
+      void validateOutput(AWS.Cryptography.KeyStore.GetItemsForInitializeMutationOutput nativeOutput)
+      {
+        try { nativeOutput.Validate(); }
+        catch (ArgumentException e)
+        {
+          var message = $"Output of {_impl}._GetItemsForInitializeMutation is invalid. {e.Message}";
+          throw new KeyStoreException(message);
+        }
+      }
+      AWS.Cryptography.KeyStore.GetItemsForInitializeMutationInput nativeInput = TypeConversion.FromDafny_N3_aws__N12_cryptography__N8_keyStore__S34_GetItemsForInitializeMutationInput(input);
+      try
+      {
+        AWS.Cryptography.KeyStore.GetItemsForInitializeMutationOutput nativeOutput = _impl.GetItemsForInitializeMutation(nativeInput);
+        _ = nativeOutput ?? throw new KeyStoreException($"{_impl}._GetItemsForInitializeMutation returned null, should be {typeof(AWS.Cryptography.KeyStore.GetItemsForInitializeMutationOutput)}");
+        validateOutput(nativeOutput);
+        return Wrappers_Compile.Result<software.amazon.cryptography.keystore.internaldafny.types._IGetItemsForInitializeMutationOutput, software.amazon.cryptography.keystore.internaldafny.types._IError>.create_Success(TypeConversion.ToDafny_N3_aws__N12_cryptography__N8_keyStore__S35_GetItemsForInitializeMutationOutput(nativeOutput));
+      }
+      catch (Exception e)
+      {
+        return Wrappers_Compile.Result<software.amazon.cryptography.keystore.internaldafny.types._IGetItemsForInitializeMutationOutput, software.amazon.cryptography.keystore.internaldafny.types._IError>.create_Failure(TypeConversion.ToDafny_CommonError(e));
+      }
+    }
+    public Wrappers_Compile._IResult<software.amazon.cryptography.keystore.internaldafny.types._IGetItemsForInitializeMutationOutput, software.amazon.cryptography.keystore.internaldafny.types._IError> GetItemsForInitializeMutation_k(software.amazon.cryptography.keystore.internaldafny.types._IGetItemsForInitializeMutationInput input)
+    {
+      throw new KeyStoreException("Not supported at this time.");
+    }
     public Wrappers_Compile._IResult<software.amazon.cryptography.keystore.internaldafny.types._IWriteNewEncryptedBranchKeyVersionOutput, software.amazon.cryptography.keystore.internaldafny.types._IError> WriteNewEncryptedBranchKeyVersion(software.amazon.cryptography.keystore.internaldafny.types._IWriteNewEncryptedBranchKeyVersionInput input)
     {
       void validateOutput(AWS.Cryptography.KeyStore.WriteNewEncryptedBranchKeyVersionOutput nativeOutput)
@@ -98,6 +182,34 @@ namespace AWS.Cryptography.KeyStore
       }
     }
     public Wrappers_Compile._IResult<software.amazon.cryptography.keystore.internaldafny.types._IWriteNewEncryptedBranchKeyVersionOutput, software.amazon.cryptography.keystore.internaldafny.types._IError> WriteNewEncryptedBranchKeyVersion_k(software.amazon.cryptography.keystore.internaldafny.types._IWriteNewEncryptedBranchKeyVersionInput input)
+    {
+      throw new KeyStoreException("Not supported at this time.");
+    }
+    public Wrappers_Compile._IResult<software.amazon.cryptography.keystore.internaldafny.types._IQueryForVersionsOutput, software.amazon.cryptography.keystore.internaldafny.types._IError> QueryForVersions(software.amazon.cryptography.keystore.internaldafny.types._IQueryForVersionsInput input)
+    {
+      void validateOutput(AWS.Cryptography.KeyStore.QueryForVersionsOutput nativeOutput)
+      {
+        try { nativeOutput.Validate(); }
+        catch (ArgumentException e)
+        {
+          var message = $"Output of {_impl}._QueryForVersions is invalid. {e.Message}";
+          throw new KeyStoreException(message);
+        }
+      }
+      AWS.Cryptography.KeyStore.QueryForVersionsInput nativeInput = TypeConversion.FromDafny_N3_aws__N12_cryptography__N8_keyStore__S21_QueryForVersionsInput(input);
+      try
+      {
+        AWS.Cryptography.KeyStore.QueryForVersionsOutput nativeOutput = _impl.QueryForVersions(nativeInput);
+        _ = nativeOutput ?? throw new KeyStoreException($"{_impl}._QueryForVersions returned null, should be {typeof(AWS.Cryptography.KeyStore.QueryForVersionsOutput)}");
+        validateOutput(nativeOutput);
+        return Wrappers_Compile.Result<software.amazon.cryptography.keystore.internaldafny.types._IQueryForVersionsOutput, software.amazon.cryptography.keystore.internaldafny.types._IError>.create_Success(TypeConversion.ToDafny_N3_aws__N12_cryptography__N8_keyStore__S22_QueryForVersionsOutput(nativeOutput));
+      }
+      catch (Exception e)
+      {
+        return Wrappers_Compile.Result<software.amazon.cryptography.keystore.internaldafny.types._IQueryForVersionsOutput, software.amazon.cryptography.keystore.internaldafny.types._IError>.create_Failure(TypeConversion.ToDafny_CommonError(e));
+      }
+    }
+    public Wrappers_Compile._IResult<software.amazon.cryptography.keystore.internaldafny.types._IQueryForVersionsOutput, software.amazon.cryptography.keystore.internaldafny.types._IError> QueryForVersions_k(software.amazon.cryptography.keystore.internaldafny.types._IQueryForVersionsInput input)
     {
       throw new KeyStoreException("Not supported at this time.");
     }
