AwsCryptographicMaterialProviders/dafny/AwsCryptographyKeyStore/test/Storage/TestGetItemsForInitializeMutation.dfy
@@ -1,0 +1,82 @@
+// Copyright Amazon.com Inc. or its affiliates. All Rights Reserved.
+// SPDX-License-Identifier: Apache-2.0
+
+include "../Fixtures.dfy"
+
+module {:options "/functionSyntax:4"} TestGetItemsForInitializeMutation {
+  import UInt = Fixtures.UInt
+  import Types = Fixtures.Types
+  import UTF8 = Fixtures.UTF8
+  import opened Wrappers
+  import DefaultKeyStorageInterface
+  import Fixtures
+  import Structure
+  import DDB = Com.Amazonaws.Dynamodb
+  import KMS = Com.Amazonaws.Kms
+  import KeyStore
+
+  const physicalName: DDB.Types.TableName := Fixtures.branchKeyStoreName
+  const logicalName := Fixtures.logicalKeyStoreName
+  // The Key Store will consider this mutation lock invalid
+  // The Storage layer will not.
+  const mLockedId := "test-get-items-for-initialize-mutation"
+
+  method {:test} TestHappyCase()
+  {
+    // var underTest :- expect Fixtures.defaultStorage();
+    var ddbClient :- expect DDB.DynamoDBClient();
+    // The next two assumes are tragic
+    assume {:axiom} UTF8.Encode(physicalName).Success? && UTF8.EncodeAscii(physicalName) == UTF8.Encode(physicalName).value;
+    assume {:axiom} UTF8.Encode(logicalName).Success? && UTF8.EncodeAscii(logicalName) == UTF8.Encode(logicalName).value;
+    var underTest := new DefaultKeyStorageInterface.DynamoDBKeyStorageInterface(
+      ddbTableName := physicalName,
+      ddbClient := ddbClient,
+      logicalKeyStoreName := logicalName,
+      ddbTableNameUtf8 := UTF8.EncodeAscii(physicalName),
+      logicalKeyStoreNameUtf8 := UTF8.EncodeAscii(logicalName)
+    );
+    var input := Types.GetItemsForInitializeMutationInput(
+      Identifier := Fixtures.branchKeyId
+    );
+    var output :- expect underTest.GetItemsForInitializeMutation(input);
+    expect
+      output.activeItem.Type.ActiveHierarchicalSymmetricVersion?,
+      "activeItem was not Active? 'type': " + output.activeItem.EncryptionContext[Structure.TYPE_FIELD];
+    expect
+      output.beaconItem.Type.ActiveHierarchicalSymmetricBeacon?,
+      "beaconItem was not Beacon? 'type': " + output.beaconItem.EncryptionContext[Structure.TYPE_FIELD];
+    expect
+      output.mutationLock.None?,
+      "MutationLock was not None. 'UUID': " + output.mutationLock.value.UUID;
+  }
+
+  method {:test} TestHappyCaseMLocked()
+  {
+    // var underTest :- expect Fixtures.defaultStorage();
+    // The next two assumes are tragic
+    assume {:axiom} UTF8.Encode(physicalName).Success? && UTF8.EncodeAscii(physicalName) == UTF8.Encode(physicalName).value;
+    assume {:axiom} UTF8.Encode(logicalName).Success? && UTF8.EncodeAscii(logicalName) == UTF8.Encode(logicalName).value;
+    var ddbClient :- expect DDB.DynamoDBClient();
+    var underTest := new DefaultKeyStorageInterface.DynamoDBKeyStorageInterface(
+      ddbTableName := physicalName,
+      ddbClient := ddbClient,
+      logicalKeyStoreName := logicalName,
+      ddbTableNameUtf8 := UTF8.EncodeAscii(physicalName),
+      logicalKeyStoreNameUtf8 := UTF8.EncodeAscii(logicalName)
+    );
+    var input := Types.GetItemsForInitializeMutationInput(
+      Identifier := mLockedId
+    );
+    var output :- expect underTest.GetItemsForInitializeMutation(input);
+
+    expect
+      output.activeItem.Type.ActiveHierarchicalSymmetricVersion?,
+      "activeItem was not Active? 'type': " + output.activeItem.EncryptionContext[Structure.TYPE_FIELD];
+    expect
+      output.beaconItem.Type.ActiveHierarchicalSymmetricBeacon?,
+      "beaconItem was not Beacon? 'type': " + output.beaconItem.EncryptionContext[Structure.TYPE_FIELD];
+    expect
+      output.mutationLock.Some?,
+      "MutationLock was not Some.";
+  }
+}
